Implement and verify int encoding

src/Dafny/int.dfy
@@ -4,16 +4,17 @@ Experiment with little-endian encoding of integers.
 IronFleet has good code for this at
 https://github.com/GLaDOS-Michigan/IronFleet/blob/master/ironfleet/src/Dafny/Distributed/Impl/Common/Util.i.dfy
 */
+include "machine.s.dfy"
 
-function le_enc16(x: bv16): (bs:seq<bv8>)
+function le_enc16(x: bv16): (bs:seq<byte>)
 ensures |bs| == 2
 {
-    var b0: bv8 := (x & 0xFF) as bv8;
-    var b1: bv8 := (x >> 8) as bv8;
+    var b0: byte := (x & 0xFF) as byte;
+    var b1: byte := (x >> 8) as byte;
     [b0, b1]
 }
 
-function le_dec16(x: seq<bv8>): bv16
+function le_dec16(x: seq<byte>): bv16
 requires |x| == 2
 {
     (x[0] as bv16) |
@@ -28,9 +29,9 @@ ensures le_dec16(le_enc16(x)) == x
 }
 */
 
-function {:axiom} le_enc64(x: bv64): (bs:seq<bv8>)
+function method {:axiom} le_enc64(x: uint64): (bs:seq<byte>)
 ensures |bs| == 8
-function {:axiom} le_dec64(bs: seq<bv8>): bv64
+function method {:axiom} le_dec64(bs: seq<byte>): uint64
 requires |bs| == 8
-lemma {:axiom} lemma_le_enc_dec64(x: bv64)
+lemma {:axiom} lemma_le_enc_dec64(x: uint64)
 ensures le_dec64(le_enc64(x)) == x
