src/Dafny/machine.s.dfy
@@ -1,0 +1,2 @@
+type byte = bv8
+type uint64 = x:int | x < 0x1_0000_0000_0000_0000
