src/Dafny/marshal.dfy
@@ -1,0 +1,103 @@
+include "machine.s.dfy"
+include "int.dfy"
+
+datatype Encodable = EncUInt64(x:uint64)
+
+function enc_encode(e: Encodable): seq<byte>
+{
+    match e
+    case EncUInt64(x) => le_enc64(x)
+}
+
+function seq_encode(es: seq<Encodable>): seq<byte>
+decreases es
+{
+    if es == [] then []
+    else enc_encode(es[0]) + seq_encode(es[1..])
+}
+
+lemma {:induction es1} seq_encode_app(es1: seq<Encodable>, es2: seq<Encodable>)
+ensures seq_encode(es1 + es2) == seq_encode(es1) + seq_encode(es2)
+{
+    if es1 == [] {
+        assert es1 + es2 == es2;
+    } else {
+        //assert seq_encode([es1[0]]) == enc_encode(es1[0]);
+        //assert seq_encode(es1[1..] + es2) == seq_encode(es1[1..] + es2);
+        //assert seq_encode(es1) == enc_encode(es1[0]) + seq_encode(es1[1..]);
+        assert es1 + es2 == [es1[0]] + es1[1..] + es2;
+        assert ([es1[0]] + es1[1..] + es2)[0] == es1[0];
+        // NOTE(tej): discovered with a calc statement
+        assert ([es1[0]] + es1[1..] + es2)[1..] == es1[1..] + es2;
+    }
+}
+
+predicate prefix_of<T>(s1: seq<T>, s2: seq<T>) {
+    |s1| <= |s2| && s1 == s2[..|s1|]
+}
+
+lemma prefix_of_concat2<T>(s1: seq<T>, s2: seq<T>, s: seq<T>)
+requires prefix_of(s1, s2)
+ensures prefix_of(s1, s2 + s)
+{
+}
+
+lemma prefix_of_refl<T>(s: seq<T>)
+ensures prefix_of(s, s)
+{
+}
+
+lemma prefix_of_refl_inv<T>(s1: seq<T>, s2: seq<T>)
+requires prefix_of(s1, s2)
+requires |s1| == |s2|
+ensures s1 == s2
+{
+}
+
+class {:autocontracts} Encoder
+{
+    ghost var enc: seq<Encodable>;
+    ghost const size: nat;
+    var data: array<byte>;
+    var off: nat;
+
+    predicate Valid()
+    {
+        && off <= data.Length
+        && seq_encode(enc) == data[..off]
+        && data.Length == size
+    }
+
+    constructor(size: nat)
+    {
+        this.data := new byte[size];
+        this.off := 0;
+        this.enc := [];
+        this.size := size;
+    }
+
+    function bytes_left(): nat
+    requires Valid()
+    {
+        data.Length-off
+    }
+
+    method EncInt(x: uint64)
+    requires bytes_left() >= 8
+    {
+        forall k: nat | 0 <= k < 8 {
+            data[off+k] := le_enc64(x)[k];
+        }
+        assert data[off..off+8] == le_enc64(x);
+        off := off + 8;
+        enc := enc + [EncUInt64(x)];
+        seq_encode_app(old(enc), [EncUInt64(x)]);
+    }
+
+    method Finish() returns (bs:array<byte>)
+    ensures prefix_of(seq_encode(enc), bs[..])
+    ensures bs.Length == size
+    {
+        return data;
+    }
+}
